Crypto.v
@@ -1,0 +1,445 @@
+(** 
+Perfect Crypto - Simple definitions for message encryption and signing using
+symmetric and assymetric keys
+
+Perry Alexander
+The University of Kansas
+
+Provides definitions for:
+
+- [keyType] - [symmetric], [public] and [private] key constructors.
+- [inverse] - defines the inverse of any key.
+- [is_inverse] - proof that [inverse] is decidable and provides a decision procesure for [inverse].
+- [is_not_decryptable] - predicate indicating that a message is or is not decryptable using a specified key.
+- [decrypt] - attempts to decrypt a message with a given key.  Returns the decrypted message if decryption occurs.  Returns a proof that the message cannot be decrypted with the key if decryption does not occur.
+- [is_signed] - proof that signature checking is decidable and provides a decision procedure for signature check.
+- [check] - checks a signature on a message with a given key.  Returns a proof that the check succeeds or does not succeed.
+- [check_dec] - proof that signature checking is decidable and provides a decision procedure for signature checking.  Alternative function for [check].
+*)
+
+Require Import Omega.
+Require Import Ensembles.
+Require Import CpdtTactics.
+Require Import Eqdep_dec.
+Require Import Peano_dec.
+Require Import Coq.Program.Equality.
+
+(** Ltac helper functions for discharging cases generated from sumbool types
+  using one or two boolean cases. *)
+
+Ltac eq_not_eq P := destruct P;
+  [ (left; subst; reflexivity) |
+    (right; unfold not; intros; inversion H; contradiction) ].
+
+Ltac eq_not_eq' P Q := destruct P; destruct Q;
+  [ (subst; left; reflexivity) |
+    (right; unfold not; intros; inversion H; contradiction) |
+    (right; unfold not; intros; inversion H; contradiction) |
+    (right; unfold not; intros; inversion H; contradiction) ].
+
+(** Key values will be [nat] by default.  Could be anything satisfying
+ properties following.  *)
+
+Definition key_val : Type := nat.
+
+(** Key types are [symmetric], [public] and [private]. *)
+Inductive keyType: Type :=
+| symmetric : key_val -> keyType
+| private : key_val -> keyType
+| public : key_val -> keyType.
+
+(** A [symmetric] key is its own inverse.  A [public] key is the inverse of
+  the [private] key with the same [key_val].  A [private] key is the inverse of
+  the [public] key with the same [key_val]. *)
+
+Fixpoint inverse(k:keyType):keyType :=
+match k with
+| symmetric k => symmetric k
+| public k => private k
+| private k => public k
+end.
+
+(** Proof that inverse is decidable for any two keys. The resulting proof
+ gives us the function [is_inverse] that is a decision procedure for key 
+ inverse checking.  It will be used in [decrypt] and [check] later in the
+ specification. *)
+
+Theorem is_inverse:forall k k', {k = (inverse k')}+{k <> (inverse k')}.
+Proof.
+  intros.
+  destruct k; destruct k';
+  match goal with
+  | [ |- {symmetric ?P = (inverse (symmetric ?Q))}+{symmetric ?P <> (inverse (symmetric ?Q))} ] => (eq_not_eq (eq_nat_dec P Q))
+  | [ |- {private ?P = (inverse (public ?Q))}+{private ?P <> (inverse (public ?Q))} ] => (eq_not_eq (eq_nat_dec P Q))
+  | [ |- {public ?P = (inverse (private ?Q))}+{public ?P <> (inverse (private ?Q))} ] => (eq_not_eq (eq_nat_dec P Q))
+  | [ |- _ ] => right; simpl; unfold not; intros; inversion H
+  end.
+Defined.
+
+Eval compute in (is_inverse (public 1) (private 1)).
+
+Eval compute in (is_inverse (public 1) (private 2)).
+
+Eval compute in (is_inverse (public 2) (private 1)).
+
+Eval compute in (is_inverse (private 1) (public 1)).
+
+Eval compute in (is_inverse (symmetric 1) (symmetric 1)).
+
+Eval compute in (is_inverse (symmetric 1) (symmetric 2)).
+
+(** Various proofs for keys and properties of the inverse operation.  All keys
+  must have an inverse.  All keys have a unique inverse.  Equal inverses come
+  from equal keys *)
+
+Theorem inverse_injective : forall k1 k2, inverse k1 = inverse k2 -> k1 = k2.
+Proof.
+  intros.
+  destruct k1; destruct k2; simpl in H; try (inversion H); try (reflexivity).
+Qed.
+
+Hint Resolve inverse_injective.
+
+Theorem inverse_inverse : forall k, inverse (inverse k) = k.
+Proof.
+  intros. destruct k; try reflexivity.
+Qed.
+
+Hint Resolve inverse_inverse.
+
+Theorem inverse_surjective : forall k, exists k', (inverse k) = k'.
+Proof.
+  intros. exists (inverse k). auto.
+Qed.
+
+Hint Resolve inverse_surjective.
+
+Theorem inverse_bijective : forall k k',
+    inverse k = inverse k' ->
+    k = k' /\ forall k, exists k'', inverse k = k''.
+Proof.
+  auto.
+Qed.
+
+Inductive type : Type :=
+| Basic : type
+| Key : type
+| Encrypt : type -> type
+| Hash : type -> type
+| Pair : type -> type -> type.
+
+(** Basic messages are natural numbers.  Really should be held abstract, but we
+  need an equality decision procedure to determine message equality.  Compound 
+  messages are keys, encrypted messages, hashes and pairs. Note that signed
+  messages are pairs of a message and encrypted hash. *) 
+
+Inductive message : type -> Type :=
+| basic : nat -> message Basic
+| key : keyType -> message Key
+| encrypt : forall t, message t -> keyType -> message (Encrypt t)
+| hash : forall t, message t -> message (Hash t)
+| pair : forall t1 t2, message t1 -> message t2 -> message (Pair t1 t2).
+
+(** Predicate that determines if a message cannot be decrypted.  Could be
+  that it is not encrypted to begin with or the wrong key is used. *)
+
+Definition is_not_decryptable{t:type}(m:message t)(k:keyType):Prop :=
+  match m with
+  | encrypt t m' k' => k <> inverse k'
+  | _ => True
+  end.
+
+Definition is_decryptable{t:type}(m:message t)(k:keyType):Prop :=
+  match m with
+  | encrypt t m' k' => k = inverse k'
+  | _ => False
+  end.
+
+(** Prove that is_not_decryptable and is_decryptable are inverses.  This is a
+  bit sloppy.  Should really only have one or the other, but this theorem
+  assures they play together correctly.  Note that it is not installed as
+  a Hint.  *)
+
+Theorem decryptable_inverse: forall t:type, forall m:(message t), forall k,
+    (is_not_decryptable m k) <-> not (is_decryptable m k).
+Proof.
+  intros.
+  split. destruct m; try (tauto).
+  simpl. intros. assumption.
+  intros. destruct m; try (reflexivity).
+  simpl. tauto.
+Qed.  
+
+(** [decrypt] returns either a decrypted message or a proof of why the message
+  cannot be decrypted.  Really should be able to shorten the proof. *)
+
+(*
+Inductive sumor (A : Type) (B : Prop) : Type :=
+    inleft : A -> A + {B} | inright : B -> A + {B}
+*)
+
+Theorem is_not_decryptable_basic: forall n k, is_not_decryptable (basic n) k.
+Proof.
+  intros.
+  reflexivity.
+Qed.
+
+Theorem is_not_decryptable_key: forall k k', is_not_decryptable (key k) k'.
+Proof.
+  intros.
+  reflexivity.
+Qed.  
+
+Theorem is_not_decryptable_hash: forall t n k, is_not_decryptable (hash t n) k.
+Proof.
+  intros.
+  reflexivity.
+Qed.
+
+Theorem is_not_decryptable_pair: forall t u n m k, is_not_decryptable (pair t u n m) k.
+Proof.
+  intros.
+  reflexivity.
+Qed.
+
+Fixpoint decrypt{t:type}(m:message (Encrypt t))(k:keyType):message t+{(is_not_decryptable m k)}.
+refine match m with encrypt t m' j => (if (is_inverse k j) then (inleft _ m') else (inright _ _ )) end.
+Proof.
+  simpl. assumption.
+Defined.  
+
+Fixpoint decrypt'{t:type}(m:message (Encrypt t))(k:keyType):message t+{(is_not_decryptable m k)}.
+refine
+  match m with
+  | basic _ => inright _ is_not_decryptable_basic
+  | key _ => inright _ is_not_decryptable_key
+  | encrypt t m' j => (if (is_inverse k j) then (inleft _ m') else (inright _ _ ))
+  | hash _ _ => inright _ is_not_decryptable_hash
+  | pair _ _ _ _ => inright _ is_not_decryptable_pair
+  end.
+Proof.
+  simpl. assumption.
+Abort.
+
+(** This should solve the previous proof if there is a way to try it on every
+  proof generated by refine
+
+  repeat try (match goal with
+  | [ |- is_not_decryptable (encrypt ?X ?Y) ?Z ] => simpl; assumption
+  | [ |- _ ] => reflexivity
+  end).
+*)
+
+Eval compute in decrypt(encrypt Basic (basic 1) (symmetric 1)) (symmetric 1).
+
+Eval compute in decrypt(encrypt Basic (basic 1) (symmetric 1)) (symmetric 2).
+
+(** Generate a signature using encryption and hash *)
+
+Definition sign{t:type}(m:message t)(k:keyType) :=
+  (pair t (Encrypt (Hash t)) m (encrypt (Hash t) (hash t m) k)).
+
+Eval compute in sign (basic 1) (public 1).
+
+Ltac eq_key_helper :=
+  match goal with
+  | [ |- {symmetric ?P = symmetric ?Q} + {symmetric ?P <> symmetric ?Q} ] =>
+    (eq_not_eq (eq_nat_dec P Q))
+  | [ |- {public ?P = public ?Q} + {public ?P <> public ?Q} ] =>
+    (eq_not_eq (eq_nat_dec P Q))
+  | [ |- {private ?P = private ?Q} + {private ?P <> private ?Q} ] =>
+    (eq_not_eq (eq_nat_dec P Q))
+  | [ |- _ ] => right; unfold not; intros; inversion H
+  end.
+
+Theorem eq_key_dec: forall k k':keyType, {k=k'}+{k<>k'}.
+Proof.
+  intros.
+  destruct k; destruct k'; eq_key_helper.
+Defined.
+  
+Hint Resolve eq_key_dec.
+
+Theorem eq_type_dec: forall x y : type, {x = y} + {x <> y}.
+Proof.
+  induction x, y;
+  match goal with
+  | [ |- {?T = ?T} + {?T <> ?T} ] => left; reflexivity
+  | [ |- {?C ?T = ?C ?U} + {?C ?T <> ?C ?U} ] => specialize IHx with y; destruct IHx; [ left; subst; reflexivity | right; unfold not; intros; inversion H; contradiction ]
+  | [ |- {?C ?T ?U = ?C ?T' ?U'} + {?C ?T ?U <> ?C ?T' ?U'} ] => specialize IHx1 with y1; specialize IHx2 with y2; destruct IHx1; destruct IHx2; 
+  [ left; subst; reflexivity
+   | subst; right; unfold not; intros; inversion H; contradiction
+   | subst; right; unfold not; intros; inversion H; contradiction
+   | subst; right; unfold not; intros; inversion H; contradiction ]
+  | [ |- _ ] => right; unfold not; intros; inversion H 
+  end.
+  Qed.
+
+Theorem message_eq_lemma: forall t, forall m:(message t), forall m':(message t), forall k k',
+    {m=m'}+{m<>m'} ->
+    {k=k'}+{k<>k'} ->
+    {(encrypt t m k)=(encrypt t m' k')}+{(encrypt t m k) <> (encrypt t m' k')}.
+Proof.
+  intros.
+  destruct H; destruct H0.
+  left; subst; reflexivity.
+  right; subst; unfold not; intros; inversion H; contradiction.
+  right. subst. unfold not. intros. inversion H. apply inj_pair2_eq_dec in H1. contradiction.
+  apply eq_type_dec.
+  right. unfold not. intros. inversion H. apply inj_pair2_eq_dec in H1. contradiction.
+  apply eq_type_dec.
+Defined.
+
+Hint Resolve message_eq_lemma.
+
+Ltac whack_right :=
+  match goal with
+  | [ |- {basic ?P = basic ?Q}+{basic ?P <> basic ?Q} ] =>
+    (eq_not_eq (eq_nat_dec P Q))
+  | [ |- {key ?P = key ?Q}+{key ?P <> key ?Q} ] =>
+    (eq_not_eq (eq_key_dec P Q))
+  | [ |- {encrypt ?P ?P' = encrypt ?Q ?Q'}+{encrypt ?P ?P' <> encrypt ?Q ?Q'} ] =>
+    auto 
+  | [ H : {?P = ?Q}+{?P <> ?Q} |- {hash ?P = hash ?Q}+{hash ?P <> hash ?Q} ] =>
+    (eq_not_eq H)
+  | [ H1 : {?P = ?P'}+{?P <> ?P'},
+      H2 : {?Q = ?Q'}+{?Q <> ?Q'}
+      |- {pair ?P ?Q = pair ?P' ?Q'}+{pair ?P ?Q <> pair ?P' ?Q'} ] =>
+    (eq_not_eq' H1 H2)
+  | [ |- _ ] => right; unfold not; intros; inversion H
+  end.
+
+Theorem message_eq_dec: forall t, forall m:(message t), forall m':(message t), {m=m'}+{m<>m'}.
+Proof.
+  dependent induction m; dependent induction m'.
+  (eq_not_eq (eq_nat_dec n n0)).
+  (eq_not_eq (eq_key_dec k k0)).
+
+  specialize IHm with m'.
+  destruct IHm; destruct (eq_key_dec k k0);
+  [ left; subst; reflexivity
+  | right; unfold not; intros; inversion H; contradiction
+  | right; unfold not; intros; inversion H; apply inj_pair2_eq_dec in H1;
+    [contradiction | apply eq_type_dec]
+  | right; unfold not; intros; inversion H; apply inj_pair2_eq_dec in H1;
+    [contradiction | apply eq_type_dec]].
+  
+  specialize IHm with m'.
+  destruct IHm;
+  [ left; subst; reflexivity 
+  | right; unfold not; intros; inversion H; apply inj_pair2_eq_dec in H1;
+    [contradiction | apply eq_type_dec]].
+  
+  specialize IHm2 with m'2.
+  specialize IHm1 with m'1.
+  destruct IHm1; destruct IHm2;
+  [ left; subst; reflexivity 
+  | right; unfold not; intros; inversion H; apply inj_pair2_eq_dec in H1; apply inj_pair2_eq_dec in H2; [ contradiction | apply eq_type_dec | apply eq_type_dec | apply eq_type_dec ]
+  | right; unfold not; intros; inversion H; apply inj_pair2_eq_dec in H1; apply inj_pair2_eq_dec in H2; [ contradiction | apply eq_type_dec | apply eq_type_dec | apply eq_type_dec ]
+  | right; unfold not; intros; inversion H; apply inj_pair2_eq_dec in H1; apply inj_pair2_eq_dec in H2; [ contradiction | apply eq_type_dec | apply eq_type_dec | apply eq_type_dec ]].
+Defined.
+  
+
+(*
+  try (specialize (IHm m'));
+  try (specialize (IHm1 m'1));
+  try (specialize (IHm2 m'2));
+  whack_right.
+  Restart.
+  dependent induction m. dependent destruction m'.
+  destruct (eq_nat_dec n n0). subst. left; reflexivity. right; unfold not; intros; inversion H. contradiction.
+  intros m. destruct (eq_type_dec (key k) m).
+Defined.
+ *)
+
+Hint Resolve message_eq_dec.
+
+Print encrypt.
+
+(*Definition is_signed{t:type}(m:message (Pair t (Encrypt (Hash t))))(k:keyType):Prop :=
+  match m with
+  | pair t t' n n' => n' = sign n k
+  | _ => False
+  end.
+  
+  match m with
+  | (pair r (Encrypt (Hash r')) m' m'') => match (decrypt m'' k) with
+                      | inleft (hash r m''') => m'=m'''
+                      | inleft _ => False
+                      | inright _ => False
+                      end
+  | _ => False
+  end.
+
+
+
+    
+  | (pair t t' m m') => match m' with
+                       | encrypt t m'' k' =>  match m'' with
+                                            | (hash t m''') => m=m''' /\ (k = inverse k')
+                                      end
+                  end
+  end. 
+
+Example sign_1_ex: is_signed (pair (basic 1) (encrypt (hash (basic 1)) (private sf1))) (public 1).
+Proof.
+  simpl. tauto.
+Qed.
+
+Example sign_2_ex: not (is_signed (pair (basic 1) (encrypt (hash (basic 1)) (private 1))) (public 2)).
+Proof.
+  unfold not. intros.
+  simpl in H. inversion H. inversion H1.
+Qed.
+
+Theorem check_dec: forall m:message, forall k, {(is_signed m k)}+{not (is_signed m k)}.
+Proof.
+  intros.
+  destruct m; try tauto.
+  destruct m2; try tauto.
+    destruct m2; try tauto.
+      destruct (is_inverse k k0).
+        destruct (message_eq_dec m1 m2); try tauto.
+        left. subst. simpl. tauto.
+          right. unfold not. intros. simpl in H. tauto.
+          right. unfold not. intros. simpl in H. tauto.
+Defined. 
+            
+Eval compute in check_dec (sign (basic 1) (private 1)) (public 1).
+
+Eval compute in check_dec (sign (basic 1) (private 1)) (public 2).
+
+Notation " 'good' " := (left _ _).
+
+Notation " 'bad' " := (right _ _).
+
+Eval compute in check_dec (sign (basic 1) (private 1)) (public 1).
+
+Eval compute in check_dec (sign (basic 1) (private 1)) (public 2). *)
+
+Theorem m2 : forall P Q R: Prop, P -> Q -> R -> Q.
+Proof.
+  intros. match goal with | [ B : _ |- _ ] => exact B end.
+Qed.                                                 
+
+(** [notHyp] determines if [P] is in the assumption set of a proof state.
+  The first match case simply checks to see if [P] matches any assumption and
+  fails if it does.  The second match case grabs everything else.  If [P]
+  is a conjunction, it checks to see if either of its conjuncts is an
+  assumption calling [notHyp] recursively. 
+
+*)
+
+Ltac notHyp P :=
+  match goal with
+  | [ _ : P |- _ ] => fail 1
+  | _ =>
+    match P with
+    | ?P1 /\ ?P2 => first [ notHyp P1 | notHyp P2 | fail 2 ]
+    | _ => idtac
+    end
+  end.
+                           
+Ltac extend pf :=
+  let t := type of pf in
+  notHyp t; generalize pf; intro.
